FormalWeb.lean
@@ -1,4 +1,7 @@
 -- This module serves as the root of the `FormalWeb` library.
 -- Import modules here that should be built as part of the library.
-import FormalWeb.Basic
+import FormalWeb.Document
+import FormalWeb.SessionHistory
+import FormalWeb.Navigation
+import FormalWeb.Traversable
 import FormalWeb.UserAgent
